ConditionalElimination.thy
@@ -1,32 +1,34 @@
 theory ConditionalElimination
   imports
     IREval
-    Stamp
 begin
-
-fun stamp :: "IRGraph \<Rightarrow> ID \<Rightarrow> Stamp" where
-  "stamp g nid = unrestricted (IntegerStamp 8 0 0)"
 
 fun wff_stamps :: "IRGraph \<Rightarrow> bool" where
   "wff_stamps g = (\<forall> n \<in> ids g . 
-    (\<forall> v m . (g m \<turnstile> n (the (kind g n)) \<mapsto> v) \<and> valid_value (stamp g n) v))"
+    (\<forall> v m . (g m \<turnstile> n (kind g n) \<mapsto> v) \<and> valid_value (stamp g n) v))"
 
-lemma
-  assumes "joined = (join (stamp g x) (stamp g y))"
-  assumes "stamp_empty joined"
-  shows "\<nexists> v . valid_value joined v" 
-  using assms unfolding stamp_empty.simps
-  sorry
+lemma join_unequal:
+  assumes "joined = (join x_stamp y_stamp)"
+  assumes "is_stamp_empty joined"
+  shows "\<nexists> x y . x = y \<and> valid_value x_stamp x \<and> valid_value y_stamp y"
+  using assms disjoint_empty by auto
 
 lemma foldBinaryOpLogicJoin:
   assumes "wff_stamps g"
-  assumes "is_IntegerStamp (stamp g x)"
-  assumes "is_IntegerStamp (stamp g y)"
-  assumes "kind g nid = (Some (IntegerEqualsNode x y))"
-  assumes "g m \<turnstile> nid (the (kind g nid)) \<mapsto> v"
-  assumes "stamp_empty (join (stamp g x) (stamp g y))"
-  shows "v = IntVal 0"
-  using eval.IntegerEqualsNode
+  assumes "kind g nid = (IntegerEqualsNode x y)"
+  assumes "g m \<turnstile> nid (kind g nid) \<mapsto> v"
+  assumes "is_stamp_empty (join (stamp g x) (stamp g y))"
+  shows "v = IntVal 1 0"
+  using assms eval.IntegerEqualsNode join_unequal
+  by fastforce
 
+(*
+lemma rewriteBinaryOpLogicJoin:
+  assumes "wff_stamps g"
+  assumes "kind g1 if = (IfNode cond t f)"
+  assumes "kind g1 cond = (IntegerEqualsNode x y)"
+  assumes "is_stamp_empty (join (stamp g x) (stamp g y))"
+  shows "?"
+*)
 
 end
