Values.thy
@@ -1,0 +1,20 @@
+theory Values
+  imports
+    "HOL-Word.Word"
+    "HOL-Library.Float"
+begin
+
+type_synonym objref = "nat option"
+
+datatype UnstampedValue =
+  UnstampedFloat (uv_m: int) (uv_e: int) |
+  UnstampedInt (uv_i: int) |
+  UnstampedObj (uv_n: objref)
+
+datatype Value  =
+  UndefVal |
+  IntVal (v_bits: int) (v_int: int) |
+  FloatVal (v_bits: int) (v_float: float) |
+  ObjRef objref
+
+end
